end2end/src/end2end/KamiRiscvWordProperties.v
@@ -1,0 +1,134 @@
+Require Import Coq.ZArith.ZArith.
+Require Import coqutil.Word.Interface coqutil.Word.Properties.
+Require Import coqutil.Z.BitOps.
+Require Import coqutil.Z.Lia.
+Require Import coqutil.Tactics.destr.
+Require Import compiler.RiscvWordProperties.
+Require Import compiler.ZLemmas.
+Require Import processor.KamiWord.
+
+Open Scope Z_scope.
+
+Section KamiRiscvWord.
+  Context {log2width: Z}.
+  Context (log2width_nonneg: 0 <= log2width).
+
+  Context (width_nonneg: 0 < 2 ^ log2width).
+
+  Instance kami_word_ok: word.ok (KamiWord.word (2 ^ log2width)) := KamiWord.ok _ width_nonneg.
+
+  Arguments Z.mul: simpl never.
+
+  Instance kami_word_riscv_ok: word.riscv_ok (KamiWord.word (2 ^ log2width)).
+    constructor;
+      intros;
+      unfold word.sru, word.slu, word.srs, word.mulhuu, word.divu, word.modu, KamiWord.word.
+
+    - pose proof (word.unsigned_range y) as R1.
+      pose proof (word.unsigned_range z) as R2.
+      unfold word.unsigned in *. cbn in *.
+      remember (kunsigned y) as a. remember (kunsigned z) as b. clear Heqa Heqb y z.
+      change kunsigned with (@word.unsigned _ (KamiWord.word (2 ^ log2width))).
+      change kofZ with (@word.of_Z _ (KamiWord.word (2 ^ log2width))) at 2.
+      rewrite word.unsigned_of_Z. unfold word.wrap.
+      rewrite Z.log2_pow2 by assumption.
+      rewrite mod_mod_remove_inner.
+      + rewrite Z.mod_mod. 1: reflexivity.
+        apply Z.pow_nonzero. 1: congruence. assumption.
+      + split; [assumption|].
+        apply Z.pow_gt_lin_r; blia.
+      + apply Z.mod_divide.
+        * apply Z.pow_nonzero. 1: congruence. assumption.
+        * unfold Z.divide.
+          exists (2 ^ (2 ^ log2width - log2width)).
+          rewrite <- Z.pow_add_r.
+          { f_equal. blia. }
+          { pose proof (Z.pow_gt_lin_r 2 log2width). blia. }
+          { blia. }
+
+    - pose proof (word.unsigned_range y) as R1.
+      pose proof (word.unsigned_range z) as R2.
+      unfold word.unsigned in *. cbn in *.
+      remember (kunsigned y) as a. remember (kunsigned z) as b. clear Heqa Heqb y z.
+      change kunsigned with (@word.unsigned _ (KamiWord.word (2 ^ log2width))).
+      change kofZ with (@word.of_Z _ (KamiWord.word (2 ^ log2width))) at 2.
+      rewrite word.unsigned_of_Z. unfold word.wrap.
+      rewrite Z.log2_pow2 by assumption.
+      rewrite mod_mod_remove_inner.
+      + rewrite Z.mod_mod. 1: reflexivity.
+        apply Z.pow_nonzero. 1: congruence. assumption.
+      + split; [assumption|].
+        apply Z.pow_gt_lin_r; blia.
+      + apply Z.mod_divide.
+        * apply Z.pow_nonzero. 1: congruence. assumption.
+        * unfold Z.divide.
+          exists (2 ^ (2 ^ log2width - log2width)).
+          rewrite <- Z.pow_add_r.
+          { f_equal. blia. }
+          { pose proof (Z.pow_gt_lin_r 2 log2width). blia. }
+          { blia. }
+
+    - pose proof (word.signed_range y) as R1.
+      pose proof (word.unsigned_range z) as R2.
+      unfold word.signed, word.unsigned in *. cbn in *.
+      remember (ksigned y) as a. remember (kunsigned z) as b. clear Heqa Heqb y z.
+      change kunsigned with (@word.unsigned _ (KamiWord.word (2 ^ log2width))).
+      change kofZ with (@word.of_Z _ (KamiWord.word (2 ^ log2width))) at 2.
+      rewrite word.unsigned_of_Z. unfold word.wrap.
+      rewrite Z.log2_pow2 by assumption.
+      rewrite mod_mod_remove_inner.
+      + rewrite Z.mod_mod. 1: reflexivity.
+        apply Z.pow_nonzero. 1: congruence. assumption.
+      + split; [assumption|].
+        apply Z.pow_gt_lin_r; blia.
+      + apply Z.mod_divide.
+        * apply Z.pow_nonzero. 1: congruence. assumption.
+        * unfold Z.divide.
+          exists (2 ^ (2 ^ log2width - log2width)).
+          rewrite <- Z.pow_add_r.
+          { f_equal. blia. }
+          { pose proof (Z.pow_gt_lin_r 2 log2width). blia. }
+          { blia. }
+
+    - change kofZ with (@word.of_Z _ (KamiWord.word (2 ^ log2width))).
+      apply word.of_Z_inj_mod.
+      rewrite bitSlice_alt; cycle 1. {
+        pose proof (Z.pow_gt_lin_r 2 log2width). blia.
+      }
+      unfold bitSlice'.
+      pose proof (word.unsigned_range y) as R1.
+      pose proof (word.unsigned_range z) as R2.
+      unfold word.unsigned in *. cbn in *.
+      remember (kunsigned y) as a. remember (kunsigned z) as b. clear Heqa Heqb y z.
+      ring_simplify (2 * 2 ^ log2width - 2 ^ log2width).
+      rewrite Z.mod_mod; cycle 1. {
+        apply Z.pow_nonzero; blia.
+      }
+      reflexivity.
+
+    - unfold word.eqb.
+      match goal with
+      | |- context [ _ =? ?zero ] => replace zero with 0; cycle 1
+      end. {
+        unfold word.of_Z, kunsigned. cbn.
+        rewrite Word.wordToN_wzero'.
+        reflexivity.
+      }
+      unfold riscvZdivu.
+      destr (kunsigned z =? 0); reflexivity.
+
+    - unfold word.eqb.
+      match goal with
+      | |- context [ _ =? ?zero ] => replace zero with 0; cycle 1
+      end. {
+        unfold word.of_Z, kunsigned. cbn.
+        rewrite Word.wordToN_wzero'.
+        reflexivity.
+      }
+      unfold riscvZmodu.
+      destr (kunsigned z =? 0). 2: reflexivity.
+      rewrite <- (word.of_Z_unsigned y) at 1.
+      reflexivity.
+  Qed.
+
+End KamiRiscvWord.
